Clap/eDSLState/Writer.lean
@@ -32,6 +32,7 @@ def FixedExp.eval {p : ℕ} (varStore : ℕ → Option (ZMod p)) (x : FixedExp p
   | .sub l r => do (←eval varStore l) - (←eval varStore r)
   | .mul l r => do (←eval varStore l) * (←eval varStore r)
 
+@[grind cases]
 inductive CircuitusPlanus (p : ℕ) where
   | eq0 (e : FixedExp p)
   | lam
@@ -55,42 +56,153 @@ def CircuitStateM.run {p : ℕ} {α : Type} (cmd : CircuitStateM p α) (numAlloc
 
 structure CircuitResult (p : ℕ) where
   numAlloc : ℕ
-  varStore : Std.TreeMap ℕ (ZMod p)
+  varStore : Std.ExtTreeMap ℕ (ZMod p)
   constraints : Prop
 
-def CircuitResult.step {p : ℕ} (result : CircuitResult p) (next : CircuitusPlanus p) : CircuitResult p :=
-  let ⟨numAlloc, varStore, constraints⟩ := result
+namespace CircuitResult
+
+section
+
+variable {k : ℕ} {result result' : CircuitResult p}
+         {constraint : Prop} {vars : Vector (ZMod p) k} {e : FixedExp p}
+
+def addConstraint (result : CircuitResult p) (constraint : Prop) :=
+  {result with constraints := result.constraints ∧ constraint}
+
+@[simp, grind =]
+lemma numAlloc_addConstraint : (result.addConstraint constraint).numAlloc = result.numAlloc := rfl
+
+@[simp, grind =]
+lemma varStore_addConstraint : (result.addConstraint constraint).varStore = result.varStore := rfl
+
+@[simp, grind =]
+lemma constraints_addConstraint : (result.addConstraint constraint).constraints =
+                                  (result.constraints ∧ constraint) := rfl
+
+def allocAnonymous (result : CircuitResult p) :=
+  {result with numAlloc := result.numAlloc + 1}
+
+@[simp, grind =]
+lemma numAlloc_allocAnonymous : result.allocAnonymous.numAlloc = result.numAlloc + 1 := rfl
+
+@[simp, grind =]
+lemma varStore_allocAnonymous : result.allocAnonymous.varStore = result.varStore := rfl
+
+def get? (result : CircuitResult p) (e : FixedExp p) :=
+  e.eval result.varStore.get?
+
+@[grind =>]
+lemma get?_of_varStore_eq_varStore (h : result.varStore = result'.varStore) : result.get? e = result'.get? e := by
+  simp_all [CircuitResult.get?]
+
+def getD (result : CircuitResult p) (e : FixedExp p) :=
+  result.get? e |>.getD 0
+
+@[simp, grind =]
+lemma getD_eq_get?_getD : result.getD e = (result.get? e |>.getD 0) := rfl
+
+@[simp, grind =]
+lemma constraints_allocAnonymous : result.allocAnonymous.constraints = result.constraints := rfl
+
+def init (result : CircuitResult p) (e : FixedExp p) :=
+  result.addConstraint (result.get? e).isSome
+
+@[simp, grind =]
+lemma numAlloc_init :
+  (result.init e).numAlloc = result.numAlloc := rfl
+
+@[simp, grind =]
+lemma varStore_init :
+  (result.init e).varStore = result.varStore := rfl
+
+@[simp, grind =]
+lemma constraints_init :
+  (result.init e).constraints = (result.constraints ∧ (result.get? e).isSome = true) := rfl
+
+def alloc {k p : ℕ} (result : CircuitResult p) (vars : Vector (ZMod p) k) :=
+  let indexed := (Vector.range k).map (·+result.numAlloc) |>.zip vars
+  let varStore := result.varStore.insertMany indexed
+  {result with varStore := varStore, numAlloc := result.numAlloc + k}
+
+@[simp, grind =]
+lemma numAlloc_alloc {vars : Vector (ZMod p) k} :
+  (result.alloc vars).numAlloc = result.numAlloc + k := rfl
+
+@[simp, grind =]
+lemma varStore_alloc {vars : Vector (ZMod p) k} :
+  (result.alloc vars).varStore =
+  result.varStore.insertMany ((Vector.range k).map (·+result.numAlloc) |>.zip vars) := rfl
+
+@[simp, grind =]
+lemma constraints_alloc {vars : Vector (ZMod p) k} :
+  (result.alloc vars).constraints = result.constraints := rfl
+
+def step {p : ℕ} (result : CircuitResult p) (next : CircuitusPlanus p) : CircuitResult p :=
   match next with
-    | .eq0 e => ⟨
-      numAlloc,
-      varStore,
-      constraints ∧ (e.eval varStore.get?) = .some 0
-    ⟩
-    | .lam => ⟨
-      numAlloc + 1,
-      varStore,
-      constraints
-    ⟩
-    | .share e => ⟨
-      numAlloc + 1,
-      varStore.insert numAlloc ((e.eval varStore.get?).getD 0),
-      constraints ∧ (e.eval varStore.get?).isSome
-    ⟩
-    | .isZero e => ⟨
-      numAlloc + 1,
-      varStore.insert numAlloc (if (e.eval varStore.get?) = .some 0 then 1 else 0),
-      constraints ∧ (e.eval varStore.get?).isSome
-    ⟩
-    | .num2bits width e => ⟨
-      numAlloc + width,
-      varStore.insertMany ((Vector.range width).zip (num2bitsLsbPureV width ((e.eval varStore.get?).getD 0))),
-      constraints ∧ (e.eval varStore.get?).isSome
-    ⟩
+  | .eq0 e => result.addConstraint (result.get? e = .some 0)
+  | .lam => result.allocAnonymous
+  | .share e => result.init e |>.alloc #v[result.getD e]
+  | .isZero e => result.init e |>.alloc #v[if result.get? e = .some 0 then 1 else 0]
+  | .num2bits width e => result.init e |>.alloc (num2bitsLsbPureV width (result.getD e))
+  -- num2bits width e => ⟨
+  --   numAlloc + width,
+  --   varStore.insertMany ((Vector.range width).zip (num2bitsLsbPureV width ((e.eval varStore.get?).getD 0))),
+  --   TODO(check):         ^^^^^^^^^^^^^^^^^^^ I think we want `Vector.range width |>.map (·+numAlloc)` here,
+  --                                            and in general, in the impl. of `alloc`
+  --   constraints ∧ (e.eval varStore.get?).isSome
+  -- ⟩
 
-def CircuitState.eval {p : ℕ} (circuit : CircuitState p) (varStore : Std.TreeMap ℕ (ZMod p)) (numAlloc : ℕ) : CircuitResult p :=
-  circuit.foldl CircuitResult.step ⟨numAlloc, varStore, True⟩
+def split (result : CircuitResult p) : CircuitResult p :=
+  {result with constraints := True}
 
-lemma CircuitResult.ext {p : ℕ} {r1 r2 : CircuitResult p}
+@[simp, grind =]
+lemma numAlloc_split : result.split.numAlloc = result.numAlloc := rfl
+
+@[simp, grind =]
+lemma varStore_split : result.split.varStore = result.varStore := rfl
+
+@[simp, grind =]
+lemma constraints_split : result.split.constraints = True := rfl
+
+section
+
+variable {p width : ℕ} {result : CircuitResult p} {e : FixedExp p}
+
+@[simp, grind =]
+lemma step_eq0 :
+  result.step (.eq0 e) = result.addConstraint (result.get? e = .some 0) := rfl
+
+@[simp, grind =]
+lemma step_lam :
+  result.step .lam = result.allocAnonymous := rfl
+
+@[simp, grind =]
+lemma step_share :
+  result.step (.share e) = (result.init e |>.alloc #v[result.getD e]) := rfl
+
+@[simp, grind =]
+lemma step_isZero :
+  result.step (.isZero e) = (result.init e |>.alloc #v[if result.get? e = .some 0 then 1 else 0]) := rfl
+
+@[simp, grind =]
+lemma step_num2bits :
+  result.step (.num2bits width e) = (result.init e |>.alloc (num2bitsLsbPureV width (result.getD e))) := rfl
+
+end
+
+end
+
+end CircuitResult
+
+abbrev CircuitState.evalInOrder {p : ℕ} (circuit : CircuitState p) := circuit.foldl CircuitResult.step
+
+def CircuitState.eval {p : ℕ} (circuit : CircuitState p) (varStore : Std.ExtTreeMap ℕ (ZMod p)) (numAlloc : ℕ) : CircuitResult p :=
+  CircuitState.evalInOrder circuit ⟨numAlloc, varStore, True⟩
+
+namespace CircuitResult
+
+@[ext]
+lemma ext {p : ℕ} {r1 r2 : CircuitResult p}
   (h_numAlloc : r1.numAlloc = r2.numAlloc)
   (h_varStore : r1.varStore = r2.varStore)
   (h_constraints : r1.constraints = r2.constraints)
@@ -101,144 +213,137 @@ lemma CircuitResult.ext {p : ℕ} {r1 r2 : CircuitResult p}
   obtain ⟨a2, b2, c2⟩ := r2
   simp_all
 
-lemma CircuitResult.foldl_step_numAlloc_independent_of_constraints
+lemma foldl_step_numAlloc_independent_of_constraints
   {numAlloc : ℕ}
-  {varStore : Std.TreeMap ℕ (ZMod p)}
+  {varStore : Std.ExtTreeMap ℕ (ZMod p)}
   {constraints1 constraints2 : Prop}
   {circuit : CircuitState p}
 :
-  (circuit.foldl CircuitResult.step ⟨numAlloc, varStore, constraints1⟩).numAlloc =
-  (circuit.foldl CircuitResult.step ⟨numAlloc, varStore, constraints2⟩).numAlloc
+  (CircuitState.evalInOrder circuit ⟨numAlloc, varStore, constraints1⟩).numAlloc =
+  (CircuitState.evalInOrder circuit ⟨numAlloc, varStore, constraints2⟩).numAlloc
 := by
   obtain ⟨list⟩ := circuit
   rewrite [←List.reverse_reverse list]
-  induction list.reverse with
-    | nil =>
-      simp
-    | cons head tail h_tail =>
-      simp at h_tail
-      simp
-      set x := List.foldr _ _ _
-      set y := List.foldr _ _ _
-      cases head
-      all_goals simp [CircuitResult.step, h_tail]
+  induction list.reverse <;> grind
 
-lemma CircuitResult.foldr_step_numAlloc_independent_of_constraints
+@[grind =>]
+lemma foldr_step_numAlloc_independent_of_constraints
   {numAlloc : ℕ}
-  {varStore : Std.TreeMap ℕ (ZMod p)}
+  {varStore : Std.ExtTreeMap ℕ (ZMod p)}
   {constraints1 constraints2 : Prop}
   {circuit : List (CircuitusPlanus p)}
 :
-  (List.foldr (λ x y => CircuitResult.step y x) ⟨numAlloc, varStore, constraints1⟩ circuit).numAlloc =
-  (List.foldr (λ x y => CircuitResult.step y x) ⟨numAlloc, varStore, constraints2⟩ circuit).numAlloc
+  (List.foldr (λ x y => step y x) ⟨numAlloc, varStore, constraints1⟩ circuit).numAlloc =
+  (List.foldr (λ x y => step y x) ⟨numAlloc, varStore, constraints2⟩ circuit).numAlloc
 := by
   rewrite [←List.reverse_reverse circuit]
   simp only [List.foldr_reverse, ←List.foldl_toArray]
-  exact CircuitResult.foldl_step_numAlloc_independent_of_constraints
+  exact foldl_step_numAlloc_independent_of_constraints
 
-lemma CircuitResult.foldl_step_varStore_independent_of_constraints
+lemma foldl_step_varStore_independent_of_constraints
   {numAlloc : ℕ}
-  {varStore : Std.TreeMap ℕ (ZMod p)}
+  {varStore : Std.ExtTreeMap ℕ (ZMod p)}
   {constraints1 constraints2 : Prop}
   {circuit : CircuitState p}
 :
-  (circuit.foldl CircuitResult.step ⟨numAlloc, varStore, constraints1⟩).varStore =
-  (circuit.foldl CircuitResult.step ⟨numAlloc, varStore, constraints2⟩).varStore
+  (circuit.foldl step ⟨numAlloc, varStore, constraints1⟩).varStore =
+  (circuit.foldl step ⟨numAlloc, varStore, constraints2⟩).varStore
 := by
   obtain ⟨list⟩ := circuit
   rewrite [←List.reverse_reverse list]
-  induction list.reverse with
-    | nil =>
-      simp
-    | cons head tail h_tail =>
-      simp at h_tail
-      simp
-      set x := List.foldr _ _ _
-      set y := List.foldr _ _ _
-      have h_numAlloc : x.numAlloc = y.numAlloc := CircuitResult.foldr_step_numAlloc_independent_of_constraints
-      cases head
-      all_goals simp [CircuitResult.step, h_tail, h_numAlloc]
+  induction list.reverse <;> grind
 
-lemma CircuitResult.foldr_step_varStore_independent_of_constraints
+@[grind .]
+lemma foldr_step_varStore_independent_of_constraints
   {numAlloc : ℕ}
-  {varStore : Std.TreeMap ℕ (ZMod p)}
+  {varStore : Std.ExtTreeMap ℕ (ZMod p)}
   {constraints1 constraints2 : Prop}
   {circuit : List (CircuitusPlanus p)}
 :
-  (List.foldr (λ x y => CircuitResult.step y x) ⟨numAlloc, varStore, constraints1⟩ circuit).varStore =
-  (List.foldr (λ x y => CircuitResult.step y x) ⟨numAlloc, varStore, constraints2⟩ circuit).varStore
+  (List.foldr (λ x y => step y x) ⟨numAlloc, varStore, constraints1⟩ circuit).varStore =
+  (List.foldr (λ x y => step y x) ⟨numAlloc, varStore, constraints2⟩ circuit).varStore
 := by
   rewrite [←List.reverse_reverse circuit]
   simp only [List.foldr_reverse, ←List.foldl_toArray]
-  exact CircuitResult.foldl_step_varStore_independent_of_constraints
+  exact foldl_step_varStore_independent_of_constraints
 
-lemma CircuitResult.foldl_step_constraints_and
+/--
+This exists to appease `grind`.
+-/
+@[grind! .]
+lemma foldr_step_varStore_independent_of_constraints'
+  {circuit : List (CircuitusPlanus p)}
+  {σ₁ σ₂ : CircuitResult p}
+  (h₁ : σ₁.numAlloc = σ₂.numAlloc)
+  (h₂ : σ₁.varStore = σ₂.varStore)
+:
+  (List.foldr (λ x y => step y x) σ₁ circuit).varStore =
+  (List.foldr (λ x y => step y x) σ₂ circuit).varStore
+:= by
+  rewrite [←List.reverse_reverse circuit]
+  simp only [List.foldr_reverse, ←List.foldl_toArray]
+  grind [cases CircuitResult, foldl_step_varStore_independent_of_constraints]
+
+lemma foldl_step_constraints_and
   {result : CircuitResult p}
   {circuit : CircuitState p}
 :
-  (circuit.foldl CircuitResult.step result).constraints = (
+  (CircuitState.evalInOrder circuit result).constraints = (
     result.constraints ∧
-    (circuit.foldl CircuitResult.step ⟨result.numAlloc, result.varStore, True⟩).constraints
+    (CircuitState.evalInOrder circuit result.split).constraints
   )
 := by
   obtain ⟨list⟩ := circuit
   rewrite [←List.reverse_reverse list]
-  induction list.reverse with
-    | nil =>
-      simp
-    | cons head tail h_tail =>
-      simp at h_tail
-      simp
-      set x := List.foldr _ _ _
-      set y := List.foldr _ _ _
-      have h_varStore : x.varStore = y.varStore := CircuitResult.foldr_step_varStore_independent_of_constraints
-      cases head
-      all_goals simp [CircuitResult.step, h_tail, h_varStore, and_assoc]
+  induction list.reverse <;> grind
 
-lemma CircuitState.eval_append
+end CircuitResult
+
+namespace CircuitState
+
+@[simp, grind =]
+lemma eval_append
   {p : ℕ}
   {numAlloc}
   {circuit1 circuit2 : CircuitState p}
   {varStore}
 :
-  CircuitState.eval (circuit1 ++ circuit2) varStore numAlloc = (
-    let ⟨numAllocMid, varStoreMid, constraintsMid⟩ := CircuitState.eval circuit1 varStore numAlloc
-    let ⟨numAllocPost, varStorePost, constraintsPost⟩ := CircuitState.eval circuit2 varStoreMid numAllocMid
+  eval (circuit1 ++ circuit2) varStore numAlloc = (
+    let ⟨numAllocMid, varStoreMid, constraintsMid⟩ := eval circuit1 varStore numAlloc
+    let ⟨numAllocPost, varStorePost, constraintsPost⟩ := eval circuit2 varStoreMid numAllocMid
     ⟨numAllocPost, varStorePost, constraintsMid ∧ constraintsPost⟩
   )
 := by
-  simp [CircuitState.eval]
-  set first := Array.foldl _ _ circuit1
-  apply CircuitResult.ext
+  simp [eval]
+  ext1
   all_goals dsimp
   . exact CircuitResult.foldl_step_numAlloc_independent_of_constraints
   . exact CircuitResult.foldl_step_varStore_independent_of_constraints
   . exact CircuitResult.foldl_step_constraints_and
 
-lemma CircuitState.eval_bind
-  (α β: Type)
-  (varStore : Std.TreeMap ℕ (ZMod p))
-  (numAlloc : ℕ)
-  (action : CircuitStateM p α)
-  (function : α → CircuitStateM p β)
+@[simp, grind =]
+lemma eval_bind
+  {α β : Type}
+  {varStore : Std.ExtTreeMap ℕ (ZMod p)}
+  {numAlloc : ℕ}
+  {action : CircuitStateM p α}
+  {function : α → CircuitStateM p β}
 :
-  CircuitState.eval (CircuitStateM.run (bind action function) numAlloc).2 varStore numAlloc =
+  eval (CircuitStateM.run (action >>= function) numAlloc).2 varStore numAlloc =
   let (result, action_circuit) := action.run numAlloc
   let (_, function_circuit) := (function result).run numAlloc
-  let first_eval := CircuitState.eval action_circuit varStore numAlloc
-  let second_eval := CircuitState.eval function_circuit first_eval.varStore first_eval.numAlloc
+  let first_eval := eval action_circuit varStore numAlloc
+  let second_eval := eval function_circuit first_eval.varStore first_eval.numAlloc
   {
     numAlloc := second_eval.numAlloc
     varStore := second_eval.varStore
     constraints := first_eval.constraints ∧ second_eval.constraints
   }
 := by
-  simp [CircuitStateM.run, bind, Functor.map, ReaderT.run, WriterT.run, WriterT.mk, ReaderT.bind]
-  obtain ⟨data, state_post_action⟩ := action numAlloc
-  dsimp
-  obtain ⟨_, final_state⟩ := (function data) numAlloc
-  dsimp
-  simp [CircuitState.eval_append]
+  simp only [CircuitStateM.run, ReaderT.run, WriterT.run, bind, WriterT.mk, ReaderT.bind, Functor.map]
+  grind
+
+end CircuitState
 
 section
 
