Clap/eDSLState/Wheels.lean
@@ -1,5 +1,8 @@
 import Lean
 
+@[simp]
+theorem Vector.range_one : Vector.range 1 = #v[0] := rfl
+
 namespace Clap
 
 initialize Lean.registerTraceClass `Clap.Preprocessor
